progs/verif_bst_oo.v
@@ -392,7 +392,7 @@ Proof.
     + forward. (* p = *t; *)
       forward_if; [clear H | inversion H]. (* then clause *)
       forward_call (sizeof t_struct_tree).
-        1: simpl; rep_lia.
+        computable.
       Intros p1.
       rewrite memory_block_data_at_ by auto.
       forward. (* p->key=x; *)
