sha/verif_hmac_crypto.v
@@ -174,7 +174,7 @@ unfold data_block.
   rewrite Zlength_correct; simpl.
   rewrite <- memory_block_data_at_; trivial.
   rewrite (memory_block_data_at_ Tsh
-                    (tarray tuchar (@sizeof (@cenv_cs CompSpecs) (Tstruct _hmac_ctx_st noattr)))).
+                    (tarray tuchar (@sizeof CompSpecs (Tstruct _hmac_ctx_st noattr)))).
   2: trivial.
   eapply derives_trans. apply data_at_data_at_. apply derives_refl.
 Qed.
